<?xml version="1.0"?>
<rdf:RDF xmlns="http://www.example.com/questionTemplating#"
     xml:base="http://www.example.com/questionTemplating"
     xmlns:owl="http://www.w3.org/2002/07/owl#"
     xmlns:rdf="http://www.w3.org/1999/02/22-rdf-syntax-ns#"
     xmlns:xml="http://www.w3.org/XML/1998/namespace"
     xmlns:xsd="http://www.w3.org/2001/XMLSchema#"
     xmlns:rdfs="http://www.w3.org/2000/01/rdf-schema#"
     xmlns:terms="http://purl.org/dc/terms/">
    <owl:Ontology rdf:about="https://w3id.org/sqo">
        <terms:creator>Daniel Garijo</terms:creator>
        <terms:creator>Hernan Vargas</terms:creator>
        <terms:creator>Yolanda Gil</terms:creator>
        <terms:description>An ontology to define semantic templates for scientific questions. Defines questions, variables, options and constraints.</terms:description>
        <terms:license>https://creativecommons.org/licenses/by/2.0/</terms:license>
        <terms:title>The Scientific Questions Ontology</terms:title>
        <owl:versionInfo>v1.1.0</owl:versionInfo>
    </owl:Ontology>
    


    <!-- 
    ///////////////////////////////////////////////////////////////////////////////////////
    //
    // Annotation properties
    //
    ///////////////////////////////////////////////////////////////////////////////////////
     -->

    


    <!-- http://purl.org/dc/terms/creator -->

    <owl:AnnotationProperty rdf:about="http://purl.org/dc/terms/creator"/>
    


    <!-- http://purl.org/dc/terms/description -->

    <owl:AnnotationProperty rdf:about="http://purl.org/dc/terms/description"/>
    


    <!-- http://purl.org/dc/terms/license -->

    <owl:AnnotationProperty rdf:about="http://purl.org/dc/terms/license"/>
    


    <!-- http://purl.org/dc/terms/title -->

    <owl:AnnotationProperty rdf:about="http://purl.org/dc/terms/title"/>
    


    <!-- 
    ///////////////////////////////////////////////////////////////////////////////////////
    //
    // Object Properties
    //
    ///////////////////////////////////////////////////////////////////////////////////////
     -->

    


    <!-- https://w3id.org/sqo#hasQuestionCategory -->

    <owl:ObjectProperty rdf:about="https://w3id.org/sqo#hasQuestionCategory">
        <rdfs:domain rdf:resource="https://w3id.org/sqo#Question"/>
        <rdfs:range rdf:resource="https://w3id.org/sqo#QuestionCategory"/>
        <rdfs:comment>Link a Question with the category it belong</rdfs:comment>
        <rdfs:label>Has question category</rdfs:label>
    </owl:ObjectProperty>
    


    <!-- https://w3id.org/sqo#hasQuestionVariable -->

    <owl:ObjectProperty rdf:about="https://w3id.org/sqo#hasQuestionVariable">
        <rdfs:domain rdf:resource="https://w3id.org/sqo#Question"/>
        <rdfs:range rdf:resource="https://w3id.org/sqo#QuestionVariable"/>
        <rdfs:comment>Link a Question with all of the Question Variables that used on the question template and pattern</rdfs:comment>
        <rdfs:label>Has question variable</rdfs:label>
    </owl:ObjectProperty>
    


    <!-- 
    ///////////////////////////////////////////////////////////////////////////////////////
    //
    // Data properties
    //
    ///////////////////////////////////////////////////////////////////////////////////////
     -->

    


    <!-- https://w3id.org/sqo#hasConstraints -->

    <owl:DatatypeProperty rdf:about="https://w3id.org/sqo#hasConstraints">
        <rdfs:domain rdf:resource="https://w3id.org/sqo#QuestionVariable"/>
        <rdfs:range rdf:resource="http://www.w3.org/2001/XMLSchema#string"/>
        <rdfs:comment>An SPARQL query that will determine the options for this variable</rdfs:comment>
        <rdfs:label>Has constraints</rdfs:label>
    </owl:DatatypeProperty>
    


    <!-- https://w3id.org/sqo#hasFixedOptions -->

    <owl:DatatypeProperty rdf:about="https://w3id.org/sqo#hasFixedOptions">
        <rdfs:domain rdf:resource="https://w3id.org/sqo#QuestionVariable"/>
        <rdfs:range rdf:resource="http://www.w3.org/2001/XMLSchema#string"/>
        <rdfs:comment>List of possible options for this variable. Alternative to &quot;has contraints&quot; property</rdfs:comment>
        <rdfs:label>Has fixed options</rdfs:label>
    </owl:DatatypeProperty>
    


    <!-- https://w3id.org/sqo#hasQuestionPattern -->

    <owl:DatatypeProperty rdf:about="https://w3id.org/sqo#hasQuestionPattern">
        <rdfs:domain rdf:resource="https://w3id.org/sqo#Question"/>
        <rdfs:range rdf:resource="http://www.w3.org/2001/XMLSchema#string"/>
        <rdfs:comment>SPARQL-like pattern that defines the semantic representation that this question will have. All variables used on the question template will be replaced for the user selected values.</rdfs:comment>
        <rdfs:label>Has question pattern</rdfs:label>
    </owl:DatatypeProperty>
    


    <!-- https://w3id.org/sqo#hasQuestionTemplate -->

    <owl:DatatypeProperty rdf:about="https://w3id.org/sqo#hasQuestionTemplate">
        <rdfs:domain rdf:resource="https://w3id.org/sqo#Question"/>
        <rdfs:range rdf:resource="http://www.w3.org/2001/XMLSchema#string"/>
        <rdfs:comment>Text representation of the question that will create a form that the user must fill. All &quot;question variable&quot; names used on this template will be replaced for inputs with constraints.</rdfs:comment>
        <rdfs:label>Has question template</rdfs:label>
    </owl:DatatypeProperty>
    


    <!-- https://w3id.org/sqo#hasVariableName -->

    <owl:DatatypeProperty rdf:about="https://w3id.org/sqo#hasVariableName">
        <rdfs:domain rdf:resource="https://w3id.org/sqo#QuestionVariable"/>
        <rdfs:range rdf:resource="http://www.w3.org/2001/XMLSchema#string"/>
        <rdfs:comment>SPARQL name of this variable. Used on the question pattern and template</rdfs:comment>
        <rdfs:label>Has variable name</rdfs:label>
    </owl:DatatypeProperty>
    


    <!-- https://w3id.org/sqo#maxCardinality -->

    <owl:DatatypeProperty rdf:about="https://w3id.org/sqo#maxCardinality">
        <rdfs:domain rdf:resource="https://w3id.org/sqo#QuestionVariable"/>
        <rdfs:range rdf:resource="http://www.w3.org/2001/XMLSchema#nonNegativeInteger"/>
        <rdfs:comment>Denotes maximum cardinality for this question variable values.
As default the cardinality is 1.</rdfs:comment>
        <rdfs:label>has maximum cardinality</rdfs:label>
    </owl:DatatypeProperty>
    


    <!-- https://w3id.org/sqo#minCardinality -->

    <owl:DatatypeProperty rdf:about="https://w3id.org/sqo#minCardinality">
        <rdfs:domain rdf:resource="https://w3id.org/sqo#QuestionVariable"/>
        <rdfs:range rdf:resource="http://www.w3.org/2001/XMLSchema#nonNegativeInteger"/>
        <rdfs:comment>Denotes minimum cardinality for this question variable values.
As default the cardinality is 1.</rdfs:comment>
        <rdfs:label>has minimum cardinality</rdfs:label>
    </owl:DatatypeProperty>
    


    <!-- 
    ///////////////////////////////////////////////////////////////////////////////////////
    //
    // Classes
    //
    ///////////////////////////////////////////////////////////////////////////////////////
     -->

    


    <!-- https://w3id.org/sqo#Question -->

    <owl:Class rdf:about="https://w3id.org/sqo#Question">
        <rdfs:comment>Class that represents a scientific question. Is linked to the template, the pattern and all the variables this question uses.</rdfs:comment>
        <rdfs:label>Question</rdfs:label>
    </owl:Class>
    


    <!-- https://w3id.org/sqo#QuestionCategory -->

    <owl:Class rdf:about="https://w3id.org/sqo#QuestionCategory">
        <rdfs:comment>Class used to group together similar Questions</rdfs:comment>
        <rdfs:label>Question Category</rdfs:label>
    </owl:Class>
    


    <!-- https://w3id.org/sqo#QuestionVariable -->

    <owl:Class rdf:about="https://w3id.org/sqo#QuestionVariable">
        <rdfs:comment>Class that represents a variable used on a Question. This variable name must be present on the template and pattern of the question that uses it. Can have contraints in the form of a query (hasConstraint property) or a list of possible options (hasFixedOptions property).</rdfs:comment>
        <rdfs:label>Question Variable</rdfs:label>
    </owl:Class>
</rdf:RDF>



<!-- Generated by the OWL API (version 4.5.9.2019-02-01T07:24:44Z) https://github.com/owlcs/owlapi -->

