@prefix : <https://w3id.org/sqo#> .
@prefix owl: <http://www.w3.org/2002/07/owl#> .
@prefix rdf: <http://www.w3.org/1999/02/22-rdf-syntax-ns#> .
@prefix xml: <http://www.w3.org/XML/1998/namespace> .
@prefix xsd: <http://www.w3.org/2001/XMLSchema#> .
@prefix rdfs: <http://www.w3.org/2000/01/rdf-schema#> .
@base <https://w3id.org/sqo> .

<https://w3id.org/sqo> rdf:type owl:Ontology ;
                        <http://purl.org/dc/terms/creator> "Daniel Garijo" ,
                                                           "Hernan Vargas" ,
                                                           "Yolanda Gil" ;
                        <http://purl.org/dc/terms/description> "An ontology to define semantic templates for scientific questions. Defines questions, variables, options and constraints." ;
                        <http://purl.org/dc/terms/license> "https://creativecommons.org/licenses/by/2.0/" ;
                        <http://purl.org/dc/terms/title> "The Scientific Questions Ontology" ;
                        owl:versionInfo "v1.2.0" .

#################################################################
#    Annotation properties
#################################################################

###  http://purl.org/dc/terms/creator
<http://purl.org/dc/terms/creator> rdf:type owl:AnnotationProperty .


###  http://purl.org/dc/terms/description
<http://purl.org/dc/terms/description> rdf:type owl:AnnotationProperty .


###  http://purl.org/dc/terms/license
<http://purl.org/dc/terms/license> rdf:type owl:AnnotationProperty .


###  http://purl.org/dc/terms/title
<http://purl.org/dc/terms/title> rdf:type owl:AnnotationProperty .


#################################################################
#    Object Properties
#################################################################

###  https://w3id.org/sqo#hasQuestionCategory
:hasQuestionCategory rdf:type owl:ObjectProperty ;
                     rdfs:domain :Question ;
                     rdfs:range :QuestionCategory ;
                     rdfs:comment "Link a Question with the category it belong" ;
                     rdfs:label "Has question category" .


###  https://w3id.org/sqo#hasQuestionVariable
:hasQuestionVariable rdf:type owl:ObjectProperty ;
                     rdfs:domain :Question ;
                     rdfs:range :QuestionVariable ;
                     rdfs:comment "Link a Question with all of the Question Variables that used on the question template and pattern" ;
                     rdfs:label "Has question variable" .


#################################################################
#    Data properties
#################################################################

###  https://w3id.org/sqo#hasConstraints
:hasConstraints rdf:type owl:DatatypeProperty ;
                rdfs:domain :QuestionVariable ;
                rdfs:range xsd:string ;
                rdfs:comment "An SPARQL query that will determine the options for this variable" ;
                rdfs:label "Has constraints" .


###  https://w3id.org/sqo#hasFixedOptions
:hasFixedOptions rdf:type owl:DatatypeProperty ;
                 rdfs:domain :QuestionVariable ;
                 rdfs:range xsd:string ;
                 rdfs:comment "List of possible options for this variable. Alternative to \"has contraints\" property" ;
                 rdfs:label "Has fixed options" .


###  https://w3id.org/sqo#hasQuestionConstraint
:hasQuestionConstraint rdf:type owl:DatatypeProperty ;
                       rdfs:domain :Question ;
                       rdfs:range xsd:string ;
                       rdfs:comment "Querie that determines constraints for all variables on this Question" ;
                       rdfs:label "Has question constraint" .


###  https://w3id.org/sqo#hasQuestionPattern
:hasQuestionPattern rdf:type owl:DatatypeProperty ;
                    rdfs:domain :Question ;
                    rdfs:range xsd:string ;
                    rdfs:comment "SPARQL-like pattern that defines the semantic representation that this question will have. All variables used on the question template will be replaced for the user selected values." ;
                    rdfs:label "Has question pattern" .


###  https://w3id.org/sqo#hasQuestionTemplate
:hasQuestionTemplate rdf:type owl:DatatypeProperty ;
                     rdfs:domain :Question ;
                     rdfs:range xsd:string ;
                     rdfs:comment "Text representation of the question that will create a form that the user must fill. All \"question variable\" names used on this template will be replaced for inputs with constraints." ;
                     rdfs:label "Has question template" .


###  https://w3id.org/sqo#hasVariableName
:hasVariableName rdf:type owl:DatatypeProperty ;
                 rdfs:domain :QuestionVariable ;
                 rdfs:range xsd:string ;
                 rdfs:comment "SPARQL name of this variable. Used on the question pattern and template" ;
                 rdfs:label "Has variable name" .


###  https://w3id.org/sqo#maxCardinality
:maxCardinality rdf:type owl:DatatypeProperty ;
                rdfs:domain :QuestionVariable ;
                rdfs:range xsd:nonNegativeInteger ;
                rdfs:comment """Denotes maximum cardinality for this question variable values.
As default the cardinality is 1.""" ;
                rdfs:label "has maximum cardinality" .


###  https://w3id.org/sqo#minCardinality
:minCardinality rdf:type owl:DatatypeProperty ;
                rdfs:domain :QuestionVariable ;
                rdfs:range xsd:nonNegativeInteger ;
                rdfs:comment """Denotes minimum cardinality for this question variable values.
As default the cardinality is 1.""" ;
                rdfs:label "has minimum cardinality" .


#################################################################
#    Classes
#################################################################

###  https://w3id.org/sqo#Question
:Question rdf:type owl:Class ;
          rdfs:comment "Class that represents a scientific question. Is linked to the template, the pattern and all the variables this question uses." ;
          rdfs:label "Question" .


###  https://w3id.org/sqo#QuestionCategory
:QuestionCategory rdf:type owl:Class ;
                  rdfs:comment "Class used to group together similar Questions" ;
                  rdfs:label "Question Category" .


###  https://w3id.org/sqo#QuestionVariable
:QuestionVariable rdf:type owl:Class ;
                  rdfs:comment "Class that represents a variable used on a Question. This variable name must be present on the template and pattern of the question that uses it. Can have contraints in the form of a query (hasConstraint property) or a list of possible options (hasFixedOptions property)." ;
                  rdfs:label "Question Variable" .


###  Generated by the OWL API (version 5.1.14) https://github.com/owlcs/owlapi/
